**Dicas:**

**Tip 1:** $P (x) = a \times
 (x - x_1) \times
 (x - x_2) \times
 \ldots$
De acordo com o enunciado, $P(x) = a \times (x - 2)^2 \times (x + 1)$, no entanto, pelo Teorema do resto, $P(-3) \neq 25$.

**Tip 2:** $P (-3) = 25 \Rightarrow P (x) = a \times
 (-3 - 2)^2 \times
 (-3 + 1) = 25 \Rightarrow P (x) = a \times
 (-5)^2 \times
 (-2) = 25 \Rightarrow P (x) = a \times
 [25 \times
 (-2)] = 25 \Rightarrow a = -\frac{1}{2}$.

**Tip 3:** $P(x) = -\frac{1}{2}  (x - 2)^2 \times
 (x + 1) \Rightarrow P(x) = -\frac{1}{2}  (x^2 - 4x + 4)^2 \times
 (x + 1) \Rightarrow P(x) = -\frac{1}{2}  (x^3 - 3x^2 + 4) \Rightarrow P(x) = -x^{3/2} + \frac{3}{2}x^2 - 2$

**Opção Correta:**

$B$) $P(x) =  -x^{3/2} + \frac{3}{2}x^3 - 2$
