**Dica 1:** $\frac{6^4}{(6^3 \times 2^3) \times (6^{-3} : 2^4)}$

**Dica 2:** $\frac{6^4}{6^3 \times 2^3 \times 6^{-3} : 2^4}$

**Dica 3:** $\frac{6^4}{6^3} \times \frac{1}{2^3} \times 2^{-4} = 6^{4-3} \times 2^{-3} \times 2^{-4} = 6^1 \times 2^{-3-4} = 6 \times 2^{-7}$

Agora, calculemos o valor numérico:

$6 \times 2^{-7} = \frac{6}{2^7} = \frac{6}{128} = \frac{3}{64} = 3 \times \frac{1}{64} = 3 \times 2^{-6} = 3 \times \frac{1}{2^6} = 3 \times \frac{1}{64} = 3 \times (2^{-6}) = 3 \times (2^{-2})^3 = 3 \times (\frac{1}{4})^3 = 3 \times (\frac{1}{64}) = \frac{3}{64} = \frac{3}{2^6} = \frac{3}{2^6} = \frac{3}{64} = \frac{3}{2^6} = \frac{3}{2^6} = \frac{3}{64} = \boxed{81}$

Portanto, o valor da expressão é $81$, que corresponde à opção **C)**.
